pcuic/theories/PCUICTyping.v
@@ -1,9 +1,10 @@
 (* Distributed under the terms of the MIT license.   *)
 
 From Coq Require Import Bool String List Program BinPos Compare_dec Arith Lia.
-From MetaCoq.Template Require Import config utils Universes BasicAst AstUtils UnivSubst.
-From MetaCoq.PCUIC Require Import PCUICAst PCUICAstUtils PCUICInduction PCUICReflect
-                          PCUICLiftSubst PCUICUnivSubst PCUICEquality PCUICUtils.
+From MetaCoq.Template Require Import config utils Universes BasicAst AstUtils
+UnivSubst EnvironmentTyping.
+From MetaCoq.PCUIC Require Import PCUICAst PCUICAstUtils PCUICInduction
+PCUICReflect PCUICLiftSubst PCUICUnivSubst PCUICEquality PCUICUtils.
 
 From MetaCoq Require Export LibHypsNaming.
 
@@ -65,49 +66,8 @@ Proof.
   - rewrite IHtl app_length. simpl. lia.
 Qed.
 
-(** ** Environment lookup *)
-
-Definition global_decl_ident d :=
-  match d with
-  | ConstantDecl id _ => id
-  | InductiveDecl id _ => id
-  end.
-
-Fixpoint lookup_env (Σ : global_env) (id : ident) : option global_decl :=
-  match Σ with
-  | nil => None
-  | hd :: tl =>
-    if ident_eq id (global_decl_ident hd) then Some hd
-    else lookup_env tl id
-  end.
-
-Definition declared_constant (Σ : global_env) (id : ident) decl : Prop :=
-  lookup_env Σ id = Some (ConstantDecl id decl).
-
-Definition declared_minductive Σ mind decl :=
-  lookup_env Σ mind = Some (InductiveDecl mind decl).
-
-Definition declared_inductive Σ mdecl ind decl :=
-  declared_minductive Σ (inductive_mind ind) mdecl /\
-  List.nth_error mdecl.(ind_bodies) (inductive_ind ind) = Some decl.
-
-Definition declared_constructor Σ mdecl idecl cstr cdecl : Prop :=
-  declared_inductive Σ mdecl (fst cstr) idecl /\
-  List.nth_error idecl.(ind_ctors) (snd cstr) = Some cdecl.
-
-Definition declared_projection Σ mdecl idecl (proj : projection) pdecl : Prop :=
-  declared_inductive Σ mdecl (fst (fst proj)) idecl /\
-  List.nth_error idecl.(ind_projs) (snd proj) = Some pdecl /\
-  mdecl.(ind_npars) = snd (fst proj).
-
-(* TODO fix lookup env *)
-Lemma lookup_env_cst_inv {Σ c k cst} :
-  lookup_env Σ c = Some (ConstantDecl k cst) -> c = k.
-Proof.
-  induction Σ. simpl. discriminate.
-  simpl. destruct AstUtils.ident_eq eqn:Heq. intros [= ->]. simpl in Heq.
-  now destruct (AstUtils.ident_eq_spec c k). auto.
-Qed.
+Module PCUICLookup := Lookup PCUICTerm.
+Include PCUICLookup.
 
 (** Inductive substitution, to produce a constructors' type *)
 Definition inds ind u (l : list one_inductive_body) :=
