template-coq/theories/EnvironmentTyping.v
@@ -1,0 +1,70 @@
+From Coq Require Import Ascii String Bool OrderedType Lia List Program Arith.
+From MetaCoq.Template Require Import utils BasicAst AstUtils.
+From MetaCoq.Template Require Import Universes Environment.
+Import List.ListNotations.
+Require Import ssreflect.
+
+Set Asymmetric Patterns.
+
+Module Lookup (T : Term).
+
+  Module E := Environment T.
+
+  Import T E.
+
+  (** ** Environment lookup *)
+
+  Definition global_decl_ident d :=
+    match d with
+    | ConstantDecl id _ => id
+    | InductiveDecl id _ => id
+    end.
+
+  Fixpoint lookup_env (Σ : global_env) (id : ident) : option global_decl :=
+    match Σ with
+    | nil => None
+    | hd :: tl =>
+      if ident_eq id (global_decl_ident hd) then Some hd
+      else lookup_env tl id
+    end.
+
+  Definition declared_constant (Σ : global_env) (id : ident) decl : Prop :=
+    lookup_env Σ id = Some (ConstantDecl id decl).
+
+  Definition declared_minductive Σ mind decl :=
+    lookup_env Σ mind = Some (InductiveDecl mind decl).
+
+  Definition declared_inductive Σ mdecl ind decl :=
+    declared_minductive Σ (inductive_mind ind) mdecl /\
+    List.nth_error mdecl.(ind_bodies) (inductive_ind ind) = Some decl.
+
+  Definition declared_constructor Σ mdecl idecl cstr cdecl : Prop :=
+    declared_inductive Σ mdecl (fst cstr) idecl /\
+    List.nth_error idecl.(ind_ctors) (snd cstr) = Some cdecl.
+
+  Definition declared_projection Σ mdecl idecl (proj : projection) pdecl
+  : Prop :=
+    declared_inductive Σ mdecl (fst (fst proj)) idecl /\
+    List.nth_error idecl.(ind_projs) (snd proj) = Some pdecl /\
+    mdecl.(ind_npars) = snd (fst proj).
+
+  (* TODO fix lookup env *)
+  Lemma lookup_env_cst_inv {Σ c k cst} :
+    lookup_env Σ c = Some (ConstantDecl k cst) -> c = k.
+  Proof.
+    induction Σ. simpl. discriminate.
+    simpl. destruct AstUtils.ident_eq eqn:Heq. intros [= ->]. simpl in Heq.
+    now destruct (AstUtils.ident_eq_spec c k). auto.
+  Qed.
+
+End Lookup.
+
+Module Type Typing (T : Term).
+
+  Module E := Environment T.
+
+  Import T E.
+
+  Parameter (typing : global_env_ext -> context -> term -> term).
+
+End Typing.
